Notes & Modalities

io/LTL.fst
@@ -11,7 +11,15 @@ open IO
 (** This is based on the paper LTL Types FRP Linear-time Temporal Logic Propositions as Types by Alan Jeffrey 
     Source: https://dl.acm.org/doi/10.1145/2103776.2103783 **)
 
-(** *** Figure 1 **)
+(** *** Figure 1 -- time model **)
+(** LTL Proposition are temporal proposition, therefore we need a time model. 
+    I chose as a model for time the trace with a position.
+    What is before the position is past,
+    the position is present,
+    and what is after the position is future.
+
+    Since trace in this case is finite, there can be no future
+**)
 type time = (h:trace & (n:int{(-1 <= n /\ n < List.length h)}))
 
 let test_start_time : time = (| [], -1 |)
@@ -28,46 +36,61 @@ let has_history (| _, i |) = i > 0
 val end_time : time -> Type0
 let end_time (| h, i |) = (i+1) == List.length h
 
+(** I think here it should be prefix **)
 val time_leq : time -> time -> Type0
-let time_leq (| h1, i1 |) (| h2, i2 |) = i1 <= i2 /\ h1 == h2 // should it be = instead of prefix?
+let time_leq (| h1, i1 |) (| h2, i2 |) = h1 == h2 /\ i1 <= i2
 
 val time_lt : time -> time -> Type0
-let time_lt (| h1, i1 |) (| h2, i2 |) = i1 < i2 /\ h1 == h2
+let time_lt (| h1, i1 |) (| h2, i2 |) = h1 == h2 /\ i1 < i2
 
-// associative, cancellative, has right unit 0
+// time_sum should be associative, cancellative, has right unit 0
 unfold val time_sum : t:time -> n:int{-1 <= n+Mkdtuple2?._2 t /\ n+Mkdtuple2?._2 t < (List.length (Mkdtuple2?._1 t))} -> time 
 let time_sum (| h, i1 |) n = (| h, i1 + n |)
 
 val time_diff : t1:time -> t2:time{t2 `time_leq` t1} -> nat
 let time_diff (| _, i1 |) (| _, i2 |) = i1 - i2
 
-(** *** Figure 2 **)
+(** *** Figure 2 - type of props **)
 type ltl_prop = time -> Type0
+
+(** because we worked with prefixes until now, I add also
+    the type of prefix_prop that looks at reversed histories. **)
 type prefix_prop = trace -> Type0
+
+unfold val prefix_as_ltl : prefix_prop -> ltl_prop
+let prefix_as_ltl (p:prefix_prop) (| h, i |) =
+  i == List.length h - 1 /\
+  p (List.rev h)
+
+unfold val prefix_as_ltl' : (trace -> Tot bool) -> ltl_prop
+let prefix_as_ltl' p = prefix_as_ltl (fun h -> p h) 
 
 (** *** Effect **)
 unfold val as_time : trace -> trace -> time
 let as_time h lt = 
-  List.Tot.Properties.rev_length h;
-  (| List.rev h @ lt, List.length h - 1 |)
+  rev_length h;
+  (| rev h @ lt, length h - 1 |)
 
-effect IOltl (a:Type) (pre:prefix_prop) (post:ltl_prop) =
+(** it feels weird to have pre and post since ltl is temporal. 
+probably this is not the best encoding, but probably the fact that 
+we try to encode it in IOwp is a problem too**) 
+effect IOltl (a:Type) (pre:ltl_prop) (post:ltl_prop) =
   IO a 
-    (fun h -> pre h) 
+    (fun h -> rev_length h; pre (| (rev h), length h - 1 |)) 
     (fun h r lt -> post (as_time h lt))
 
-(** *** Figure 4 **)
+(** *** Figure 4 - temporal props over intervals **)
 val closed_interval : ltl_prop -> time -> time -> Type0
-let closed_interval p s u = forall t. s `time_leq` t ==> t `time_leq` u ==> p t // shouldn't it be /\ instead of the first ==>?
+let closed_interval p s u = forall t. s `time_leq` t ==> t `time_leq` u ==> p t
 
 val closed_open_interval : ltl_prop -> time -> time -> Type0
 let closed_open_interval p s u = forall t.  s `time_leq` t ==> t `time_lt` u ==> p t
 
-(** *** Figure 5 **)
-val yesterday : ltl_prop -> ltl_prop
-let yestarday p t =
-  has_history t /\ p (t `time_sum` (-1))
+val exists_point_in_interval : ltl_prop -> time -> time -> Type0
+let exists_point_in_interval p s u = exists t. s `time_leq` t /\ t `time_leq` u /\ p t
 
+(** *** Figure 5 - temporal modalities **)
+(** future modalities **)
 val next : ltl_prop -> ltl_prop 
 let next p t = 
   ~(end_time t) /\ p (t `time_sum` 1)
@@ -76,13 +99,36 @@ val eventually : ltl_prop -> ltl_prop
 let eventually p t = exists u. t `time_leq` u /\ p u
 
 val globally : ltl_prop -> ltl_prop
-let globally p t = forall u. t `time_leq` u /\ p t
+let globally p t = forall u. t `time_leq` u ==> p u
 
 val until : ltl_prop -> ltl_prop -> ltl_prop
-let until p q t = exists u. t `time_leq` u /\ (closed_open_interval p t u) /\ q u
+let until p q t = exists u. t `time_leq` u /\ closed_open_interval p t u /\ q u
 
 val non_strict_until : ltl_prop -> ltl_prop -> ltl_prop
-let non_strict_until p q t = exists u. t `time_leq` u /\ (closed_interval p t u) /\ q u
+let non_strict_until p q t = exists u. t `time_leq` u /\ closed_interval p t u /\ q u
+
+val constrains : ltl_prop -> ltl_prop -> ltl_prop
+let constrains p q t = forall u. t `time_leq` u ==> closed_open_interval p t u ==> q u
+
+val non_strict_constrains : ltl_prop -> ltl_prop -> ltl_prop
+let non_strict_constrains p q t = forall u. t `time_leq` u ==> closed_interval p t u ==> q u
+
+val choice : ltl_prop -> ltl_prop -> ltl_prop
+let choice p q t = forall u. t `time_leq` u ==> closed_interval p t u ==> exists_point_in_interval q t u
+
+(** past modalities **)
+val yesterday : ltl_prop -> ltl_prop
+let yestarday p t =
+  has_history t /\ p (t `time_sum` (-1))
+
+val once : ltl_prop -> ltl_prop
+let once p t = exists s. s `time_leq` t /\ p s
+
+val non_strict_since : ltl_prop -> ltl_prop -> ltl_prop
+let non_strict_since p q t = exists s. s `time_leq` t /\ closed_interval p s t /\ q s
+
+val historically : ltl_prop -> ltl_prop
+let historically p t = forall s. s `time_leq` t ==> p s
 
 (** *** Relations between primitives **)
 let next_implies_eventually (p:ltl_prop) (t:time) :
@@ -102,11 +148,11 @@ let next_implies_eventually (p:ltl_prop) (t:time) :
 
 
 (** *** Test Effect **)
-val is_closed : file_descr -> ltl_prop
-let is_closed fd (| h, i |) =
+val is_event : cmd:io_cmds -> io_sig.args cmd -> ltl_prop
+let is_event cmd arg (| h, i |) =
   0 <= i /\ i < List.length h /\
   (let e = List.Tot.index h i in
-  (EClose? e /\ EClose?.a e == fd))
+  (exists r. e == convert_call_to_event cmd arg r))
 
 val is_open_ltl : file_descr -> ltl_prop
 let is_open_ltl (fd:file_descr) t : Tot Type0 =
@@ -120,7 +166,7 @@ let is_open_ltl (fd:file_descr) t : Tot Type0 =
   end in
   f' t
 
-let lemma_index_of_append_skip (n:nat) (h lt:trace) :
+let lemma_index_of_append_skip (n:nat) (h lt:list 'a) :
   Lemma 
     (requires (n < length lt /\ List.length lt > 0))
     (ensures (
@@ -130,7 +176,7 @@ let lemma_index_of_append_skip (n:nat) (h lt:trace) :
   rev_length h;
   admit ()
 
-let lemma_index_of_append_skip_rev (n:nat) (h lt:trace) :
+let lemma_index_of_append_skip_rev (n:nat) (h lt:list 'a) :
   Lemma 
     (requires (n < length lt /\ List.length lt > 0))
     (ensures (
@@ -141,7 +187,7 @@ let lemma_index_of_append_skip_rev (n:nat) (h lt:trace) :
   rev_length h;
   lemma_index_of_append_skip 0 h lt
 
-let lemma_index_of_append_skip_0 (h lt:trace) :
+let lemma_index_of_append_skip_0 (h lt:list 'a) :
   Lemma 
     (requires (List.length lt > 0))
     (ensures (
@@ -151,28 +197,37 @@ let lemma_index_of_append_skip_0 (h lt:trace) :
     [SMTPat (index (rev h @ lt) (length h))] =
   lemma_index_of_append_skip_rev 0 h lt
 
-unfold val prefix_as_ltl : prefix_prop -> ltl_prop
-let prefix_as_ltl (p:prefix_prop) (| h, i |) =
-  i == -1 /\
-  p h
+let lemma_rev_rev (l:list 'a) :
+  Lemma (rev (rev l) == l) [SMTPat (rev (rev l))]= 
+  rev_involutive l
 
-let close (fd:file_descr) : IOltl (io_resm Close) (io_pre Close fd) (next (is_closed fd)) 
+let static_ltl_cmd (cmd:io_cmds) (arg:io_sig.args cmd) : IOltl (io_sig.res cmd arg) (prefix_as_ltl (io_pre cmd arg)) (next (is_event cmd arg)) 
   by (
   explode ();
-  bump_nth 14;
-  l_to_r [`append_nil_l;`append_l_nil];
-  let _, _ = destruct_and (nth_binder (3)) in
-  ExtraTactics.rewrite_lemma_2 (-1) 8 9;
-  rewrite (nth_binder 10);
-  let lem1 : term = `(rev_length (`#(nth_binder 1))) in
+  bump_nth 3;
+  let _, r = destruct_and (nth_binder 4) in
+  ExtraTactics.rewrite_lemma_2 (-1) 5 6;
+  rewrite (nth_binder 7);
+  let lem1 : term = `(rev_length (`#(nth_binder 2))) in
   let _ = pose_lemma lem1 in
-  let lem2 : term = `(lemma_index_of_append_skip_0 (`#(nth_binder 1)) [convert_call_to_event Close (`#(nth_binder 0)) (`#(nth_binder 9))]) in
+  let lem2 : term = `(lemma_index_of_append_skip_0 (`#(nth_binder 2)) [convert_call_to_event (`#(nth_binder 0)) (`#(nth_binder 1)) (`#(nth_binder 6))]) in
   let _ = pose_lemma lem2 in
   explode ()
   )
   =
-  static_cmd Close fd
+  static_cmd cmd arg
 
-let eventually_closed (fd:file_descr) : IOltl unit (io_pre Close fd) (eventually (is_closed fd)) =
-  let _ = close fd in
+let eventually_closed (fd:file_descr) : IOltl unit (prefix_as_ltl' (is_open fd)) (eventually (is_event Close fd)) =
+  let _ = static_ltl_cmd Close fd in
+  ()
+
+let eventually_read_closed (fd:file_descr) : IOltl unit (prefix_as_ltl' (is_open fd)) (eventually (is_event Close fd)) by (
+  explode ();
+  bump_nth 36;
+  tadmit ();
+  bump_nth 36;
+  dump "h"
+) =
+  let _ = static_ltl_cmd Read fd in
+  let _ = static_ltl_cmd Close fd in
   ()
